Veritas.SeqAux.fst
@@ -78,29 +78,29 @@ let rec proj_index_map_aux (#a:eqtype) (ss: seq a) (s: seq a) (prf:proj ss s) (i
       proj_index_map_aux ss' s' prf' i
   | PrjSkip ss' s' prf' x -> proj_index_map_aux ss' s' prf' i
 
-let proj_index_map (#a:eqtype) (ss s: seq a) (prf: proj ss s) (i: seq_index ss) = 
+let proj_index_map (#a:eqtype) (ss s: seq a) (prf: proj ss s) (i: seq_index ss) =
   proj_index_map_aux ss s prf i
 
 (* the mapping we construct above is monotonic *)
 let rec lemma_proj_monotonic_aux (#a:eqtype) (ss s: seq a) (prf: proj ss s) (i1 i2: seq_index ss):
   Lemma (requires (i1 < i2))
-        (ensures (proj_index_map ss s prf i1 < proj_index_map ss s prf i2)) 
-        (decreases prf) = 
+        (ensures (proj_index_map ss s prf i1 < proj_index_map ss s prf i2))
+        (decreases prf) =
   match prf with
-  | PrjIncl ss' s' prf' _ -> 
+  | PrjIncl ss' s' prf' _ ->
     if i2 = length ss - 1 then ()
     else lemma_proj_monotonic_aux ss' s' prf' i1 i2
   | PrjSkip ss' s' prf' _ -> lemma_proj_monotonic_aux ss' s' prf' i1 i2
 
 let lemma_proj_monotonic (#a:eqtype) (ss s: seq a) (prf: proj ss s) (i1 i2: seq_index ss):
   Lemma (requires (i1 < i2))
-        (ensures (proj_index_map ss s prf i1 < proj_index_map ss s prf i2)) = 
+        (ensures (proj_index_map ss s prf i1 < proj_index_map ss s prf i2)) =
   lemma_proj_monotonic_aux ss s prf i1 i2
 
-let rec lemma_proj_length_aux (#a:eqtype) (ss s: seq a) (prf: proj ss s): 
-  Lemma (requires (True)) 
+let rec lemma_proj_length_aux (#a:eqtype) (ss s: seq a) (prf: proj ss s):
+  Lemma (requires (True))
         (ensures (length ss <= length s))
-        (decreases prf) = 
+        (decreases prf) =
   match prf with
   | PrjEmpty -> ()
   | PrjIncl ss' s' prf' _ -> lemma_proj_length_aux ss' s' prf'
@@ -112,7 +112,7 @@ let lemma_as_squash #a #b (lem: (a -> Lemma b)) (x:a)
 
 let lemma_proj_length (#a:eqtype) (ss: seq a) (s:seq a{proj ss s}):
   Lemma (requires (True))
-        (ensures (length ss <= length s)) = 
+        (ensures (length ss <= length s)) =
   bind_squash () (lemma_as_squash #(proj ss s) #(length ss <= length s) (lemma_proj_length_aux ss s))
 
 let rec filter_aux (#a:eqtype) (f:a -> bool) (s:seq a) : Tot (seq a)
@@ -158,11 +158,11 @@ let filter_is_proj_prf (#a:eqtype) (f:a -> bool) (s: seq a) = filter_is_proj_aux
 let rec lemma_filter_correct1_aux (#a: eqtype) (f:a -> bool) (s:seq a) (i:seq_index (filter f s)):
   Lemma (requires (True))
         (ensures (f (index (filter f s) i) = true))
-        (decreases (length s)) = 
+        (decreases (length s)) =
   let n = length s in
   let fs = filter f s in
   if n = 0 then ()
-  else 
+  else
     let s' = prefix s (n - 1) in
     let e = index s (n - 1) in
     if f e then
@@ -175,12 +175,12 @@ let rec lemma_filter_correct1_aux (#a: eqtype) (f:a -> bool) (s:seq a) (i:seq_in
 let lemma_filter_correct1 (#a: eqtype) (f:a -> bool) (s:seq a) (i:seq_index (filter f s)):
   Lemma (requires (True))
         (ensures (f (index (filter f s) i) = true)) = lemma_filter_correct1_aux f s i
-        
+
 let lemma_filter_correct_all (#a:eqtype) (f:a -> bool) (s:seq a):
   Lemma (requires (True))
         (ensures (forall (i:(seq_index (filter f s))). f (index (filter f s) i) = true)) = ()
 
-let filter_index_map (#a:eqtype) (f:a -> bool) (s:seq a) (i:seq_index (filter f s)): 
+let filter_index_map (#a:eqtype) (f:a -> bool) (s:seq a) (i:seq_index (filter f s)):
   Tot (j:seq_index s{index s j = index (filter f s) i}) =
   proj_index_map (filter f s) s (filter_is_proj_prf f s) i
 
@@ -207,7 +207,7 @@ let rank_increases_by_atmost_one (#a:eqtype) (f:a -> bool) (s:seq a)
                   not (f (index s i)) && rank f s i = rank f s (i + 1))) = ()
 
 let filter_index_inv_map_aux (#a:eqtype) (f:a -> bool) (s:seq a) (i:seq_index s{f (index s i)}):
-  Tot (seq_index (filter f s)) = 
+  Tot (seq_index (filter f s)) =
   lemma_filter_len_monotonic f s (i+1);
   lemma_len_append (filter f (prefix s i)) (create 1 (index s i));
   rank f s i
@@ -215,24 +215,24 @@ let filter_index_inv_map_aux (#a:eqtype) (f:a -> bool) (s:seq a) (i:seq_index s{
 let rec lemma_filter_maps_aux (#a:eqtype) (f:a -> bool) (s:seq a) (i:seq_index s):
   Lemma (requires (f (index s i)))
         (ensures (filter_index_map f s (filter_index_inv_map_aux f s i) = i))
-        (decreases (length s)) = 
+        (decreases (length s)) =
   let n = length s in
   if n = 0 then ()
-  else 
+  else
     let s' = prefix s (n - 1) in
-    if f (index s (n - 1)) then 
+    if f (index s (n - 1)) then
       if i = n - 1 then ()
-      else 
-        lemma_filter_maps_aux f s' i          
-    else 
+      else
+        lemma_filter_maps_aux f s' i
+    else
       lemma_filter_maps_aux f s' i
 
 let filter_index_inv_map (#a:eqtype) (f:a -> bool) (s:seq a) (i:seq_index s{f (index s i)}):
-  Tot (j:seq_index (filter f s){index s i = index (filter f s) j}) = 
+  Tot (j:seq_index (filter f s){index s i = index (filter f s) j}) =
   lemma_filter_maps_aux f s i;
   filter_index_inv_map_aux f s i
 
-(* if we know that every element of a seq satisfies f, then the same sequence is a sequence over 
+(* if we know that every element of a seq satisfies f, then the same sequence is a sequence over
  * the refinement defined by f *)
 let rec seq_refine_aux (#a:Type) (f:a -> bool) (s:seq a{forall (i:seq_index s). f (index s i)})
   : Tot (seq (refine f)) (decreases (length s)) =
@@ -243,32 +243,54 @@ let rec seq_refine_aux (#a:Type) (f:a -> bool) (s:seq a{forall (i:seq_index s). 
 let seq_refine (#a:Type) (f:a -> bool) (s:seq a{all f s}): Tot (seq (refine f))
   = seq_refine_aux f s
 
-let lemma_filter_index_map_monotonic (#a:eqtype) (f:a -> bool) (s:seq a) 
+let rec lemma_seq_refine_len_aux (#a:Type) (f:a->bool) (s:seq a{all f s}):
+  Lemma (requires True)
+        (ensures (length (seq_refine f s) = length s))
+        (decreases (length s)) =
+  let n = length s in
+  if n = 0 then ()
+  else
+    lemma_seq_refine_len_aux f (prefix s (n - 1))
+
+let lemma_seq_refine_len = lemma_seq_refine_len_aux
+
+let rec lemma_seq_refine_equal_aux (#a:Type) (f:a->bool) (s:seq a{all f s}) (i:seq_index s):
+  Lemma (requires True)
+        (ensures (index (seq_refine f s) i == index s i))
+        (decreases (length s)) =
+  let n = length s in
+  if n = 0 then ()
+  else if i = n - 1 then ()
+  else lemma_seq_refine_equal_aux f (prefix s (n - 1)) i
+
+let lemma_seq_refine_equal = lemma_seq_refine_equal_aux
+
+let lemma_filter_index_map_monotonic (#a:eqtype) (f:a -> bool) (s:seq a)
   (i:seq_index (filter f s))(j:seq_index (filter f s){j > i}):
-  Lemma (filter_index_map f s i < filter_index_map f s j) = 
+  Lemma (filter_index_map f s i < filter_index_map f s j) =
   lemma_proj_monotonic (filter f s) s (filter_is_proj_prf f s) i j
 
 let lemma_filter_index_inv_map_monotonic (#a:eqtype) (f:a -> bool) (s: seq a)
   (i:seq_index s) (j: seq_index s {j > i}):
     Lemma (requires (f (index s i) /\ f (index s j)))
-          (ensures (filter_index_inv_map f s i < filter_index_inv_map f s j)) = 
+          (ensures (filter_index_inv_map f s i < filter_index_inv_map f s j)) =
   lemma_filter_len_monotonic f (prefix s j) (i+1)
 
 let lemma_filter_maps_correct (#a:eqtype) (f:a -> bool) (s: seq a) (i:seq_index s):
   Lemma (requires (f (index s i)))
-        (ensures (filter_index_map f s (filter_index_inv_map f s i) = i)) = 
+        (ensures (filter_index_map f s (filter_index_inv_map f s i) = i)) =
   lemma_filter_maps_aux f s i
 
 let lemma_filter_maps_correct2 (#a:eqtype) (f:a -> bool) (s: seq a) (i: seq_index (filter f s)):
-  Lemma (filter_index_inv_map f s (filter_index_map f s i) = i) = 
+  Lemma (filter_index_inv_map f s (filter_index_map f s i) = i) =
   let j = filter_index_map f s i in
   let i' = filter_index_inv_map f s j in
   let j' = filter_index_map f s i' in
   lemma_filter_maps_correct f s j;
-  assert(j = j');  
+  assert(j = j');
   if i < i' then
     lemma_filter_index_map_monotonic f s i i'
-  else if i > i' then 
+  else if i > i' then
     lemma_filter_index_map_monotonic f s i' i
   else ()
 
@@ -282,9 +304,9 @@ let lemma_filter_empty (#a:eqtype) (f:a -> bool):
 
 let rec lemma_filter_prefix_aux (#a:eqtype) (f:a -> bool) (s: seq a) (ps: seq a{is_prefix s ps}):
   Lemma (requires True)
-        (ensures (is_prefix (filter f s) (filter f ps))) 
+        (ensures (is_prefix (filter f s) (filter f ps)))
         (decreases (length s))
-        = 
+        =
   let n = length s in
   let fs = filter f s in
   let fps = filter f ps in
@@ -295,7 +317,7 @@ let rec lemma_filter_prefix_aux (#a:eqtype) (f:a -> bool) (s: seq a) (ps: seq a{
     let s' = prefix s (n - 1) in
     lemma_filter_prefix_aux f s' ps;
     let e = index s (n - 1) in
-    if f e then lemma_prefix_append (filter f s') (create 1 e)      
+    if f e then lemma_prefix_append (filter f s') (create 1 e)
     else ()
   )
 
@@ -303,7 +325,7 @@ let lemma_filter_prefix = lemma_filter_prefix_aux
 
 let lemma_filter_prefix_comm (#a:eqtype) (f:a->bool) (s: seq a) (i:seq_index s):
   Lemma (requires (f (index s i)))
-        (ensures (filter f (prefix s i) = prefix (filter f s) (filter_index_inv_map f s i))) = 
+        (ensures (filter f (prefix s i) = prefix (filter f s) (filter_index_inv_map f s i))) =
   lemma_filter_prefix f s (prefix s i)
 
 let lemma_filter_extend1 (#a:eqtype) (f:a -> bool) (s:seq a{length s > 0}):
@@ -318,7 +340,7 @@ let lemma_filter_extend2 (#a:eqtype) (f:a -> bool) (s:seq a{length s > 0}):
 let rec lemma_filter_extensionality_aux (#a:eqtype) (f1 f2:a -> bool) (s:seq a):
   Lemma (requires (ext_pred f1 f2))
         (ensures (filter f1 s = filter f2 s))
-        (decreases (length s)) = 
+        (decreases (length s)) =
   let n = length s in
   if n = 0 then ()
   else lemma_filter_extensionality_aux f1 f2 (prefix s (n - 1))
@@ -334,7 +356,7 @@ let rec lemma_filter_conj_aux (#a:eqtype) (f1 f2: a -> bool) (s:seq a):
   else (
     let s' = prefix s (n - 1) in
     let e = index s (n - 1) in
-    lemma_filter_conj_aux f1 f2 s';    
+    lemma_filter_conj_aux f1 f2 s';
     if conj f1 f2 e then (
       lemma_filter_extend2 (conj f1 f2) s;
       lemma_filter_extend2 f2 s;
@@ -360,7 +382,7 @@ let rec lemma_filter_conj_aux (#a:eqtype) (f1 f2: a -> bool) (s:seq a):
 let lemma_filter_conj = lemma_filter_conj_aux
 
 let lemma_filter_comm (#a:eqtype) (f1 f2:a -> bool) (s:seq a):
-  Lemma (filter f2 (filter f1 s) = filter f1 (filter f2 s)) = 
+  Lemma (filter f2 (filter f1 s) = filter f1 (filter f2 s)) =
   let cf12 = conj f1 f2 in
   let cf21 = conj f2 f1 in
   assert(ext_pred cf12 cf21);
@@ -373,13 +395,13 @@ let last_index_opt (#a:eqtype) (f:a -> bool) (s:seq a):
   let fs = filter f s in
   if length fs = 0 then None
   else Some (filter_index_map f s ((length fs) - 1))
-   
+
 let lemma_last_index_correct1 (#a:eqtype) (f:a -> bool) (s:seq a) (i:seq_index s):
   Lemma (requires (exists_sat_elems f s /\ i > last_index f s))
         (ensures (not (f (index s i)))) =
   let j = last_index f s in
   if f (index s i) then
-    lemma_filter_index_inv_map_monotonic f s j i      
+    lemma_filter_index_inv_map_monotonic f s j i
   else ()
 
 let lemma_last_index_correct2 (#a:eqtype) (f:a -> bool)  (s:seq a) (i:seq_index s):
@@ -389,8 +411,8 @@ let lemma_last_index_correct2 (#a:eqtype) (f:a -> bool)  (s:seq a) (i:seq_index 
   let ri = filter_index_inv_map f s i in
   assert (exists_sat_elems f s);
   let j = last_index f s in
-  if j < i then 
-    lemma_filter_index_inv_map_monotonic f s j i  
+  if j < i then
+    lemma_filter_index_inv_map_monotonic f s j i
   else ()
 
 let lemma_last_index_prefix (#a:eqtype) (f:a -> bool) (s:seq a) (i:nat{i <= length s}):
@@ -449,10 +471,10 @@ let lemma_last_index_last_elem_sat (#a:eqtype) (f:a -> bool) (s:seq a{length s >
 let lemma_exists_sat_elems_extensionality (#a:eqtype) (f1 f2:a -> bool) (s: seq a):
   Lemma (requires (ext_pred f1 f2))
         (ensures (exists_sat_elems f1 s = exists_sat_elems f2 s))
-        (decreases (length s)) = 
+        (decreases (length s)) =
   if exists_sat_elems f1 s then
     let i = last_index f1 s in
-    lemma_last_index_correct2 f2 s i  
+    lemma_last_index_correct2 f2 s i
   else if exists_sat_elems f2 s then
     let i = last_index f2 s in
     lemma_last_index_correct2 f1 s i
@@ -471,22 +493,22 @@ let lemma_last_index_extensionality (#a:eqtype) (f1 f2:a -> bool) (s: seq a{exis
 let lemma_exists_sat_conj (#a:eqtype) (f1 f2: a -> bool) (s: seq a):
   Lemma(requires True)
        (ensures (exists_sat_elems (conj f1 f2) s = exists_sat_elems f1 (filter f2 s)))
-       [SMTPat (exists_sat_elems (conj f1 f2) s)] = 
+       [SMTPat (exists_sat_elems (conj f1 f2) s)] =
   let s2 = filter f2 s in
-  if exists_sat_elems (conj f1 f2) s then 
+  if exists_sat_elems (conj f1 f2) s then
     let i = last_index (conj f1 f2) s in
     let j = filter_index_inv_map f2 s i in
-    lemma_last_index_correct2 f1 s2 j  
-  else if exists_sat_elems f1 s2 then 
+    lemma_last_index_correct2 f1 s2 j
+  else if exists_sat_elems f1 s2 then
     let j = last_index f1 s2 in
     let i = filter_index_map f2 s j in
-    lemma_last_index_correct2 (conj f1 f2) s i  
+    lemma_last_index_correct2 (conj f1 f2) s i
   else ()
 
-let lemma_last_idx_conj (#a:eqtype) (f1 f2: a -> bool) 
+let lemma_last_idx_conj (#a:eqtype) (f1 f2: a -> bool)
                         (s: seq a{exists_sat_elems (conj f1 f2) s}):
   Lemma (last_index (conj f1 f2) s = filter_index_map f2 s (last_index f1 (filter f2 s))) =
-  let s2 = filter f2 s in  
+  let s2 = filter f2 s in
   let i = last_index (conj f1 f2) s in
   let j = filter_index_inv_map f2 s i in
   lemma_filter_maps_correct f2 s i;
@@ -553,15 +575,15 @@ let lemma_map_index (#a #b: Type) (f:a -> b) (s:seq a) (i:seq_index s):
 
 let lemma_map_prefix (#a #b: Type) (f:a -> b) (s:seq a) (i: seq_index s):
   Lemma (requires True)
-        (ensures (map f (prefix s i) == prefix (map f s) i)) = 
+        (ensures (map f (prefix s i) == prefix (map f s) i)) =
   let mp = map f (prefix s i) in
   let pm = prefix (map f s) i in
   assert(equal mp pm);
   ()
 
 let rec zip_aux (#a #b: eqtype) (sa: seq a) (sb: seq b{length sb = length sa}):
-  Tot (sab: (seq (a * b)){length sab = length sa}) 
-  (decreases (length sa)) = 
+  Tot (sab: (seq (a * b)){length sab = length sa})
+  (decreases (length sa)) =
   let n = length sa in
   if n = 0 then empty
   else
@@ -579,20 +601,20 @@ let rec lemma_zip_index_aux (#a #b: eqtype) (sa: seq a) (sb: seq b{length sa = l
   let n = length sa in
   if n = 0 then ()
   else if i = n - 1 then ()
-  else 
+  else
     let sa' = prefix sa (n - 1) in
     let sb' = prefix sb (n - 1) in
     lemma_zip_index_aux sa' sb' i
 
 let lemma_zip_index = lemma_zip_index_aux
 
-let rec unzip_aux (#a #b: eqtype) (sab: seq (a * b)): 
+let rec unzip_aux (#a #b: eqtype) (sab: seq (a * b)):
   Tot (sasb: (seq a * seq b) {length (fst sasb) = length sab /\
                               length (snd sasb) = length sab})
-  (decreases (length sab)) = 
-  let n = length sab in 
+  (decreases (length sab)) =
+  let n = length sab in
   if n = 0 then (empty, empty)
-  else 
+  else
     let (sa',sb') = unzip_aux (prefix sab (n - 1)) in
     let (ea, eb) = index sab (n - 1) in
     (append1 sa' ea, append1 sb' eb)
@@ -603,7 +625,7 @@ let rec lemma_unzip_index_aux (#a #b: eqtype) (sab: seq (a * b)) (i:seq_index sa
   Lemma (requires (True))
         (ensures (fst (index sab i) = index (fst (unzip sab)) i /\
                   snd (index sab i) = index (snd (unzip sab)) i))
-        (decreases (length sab)) = 
+        (decreases (length sab)) =
   let n = length sab in
   if n = 0 then ()
   else if i = n - 1 then ()
@@ -619,24 +641,24 @@ let lemma_zip_unzip (#a #b: eqtype) (sa: seq a) (sb: seq b{length sb = length sa
   let sab = zip sa sb in
   assert(length sa = length (fst (unzip sab)));
   let aux1 (i:seq_index sa):
-    Lemma (requires (True)) 
+    Lemma (requires (True))
           (ensures (index sa i = index (fst (unzip sab)) i))
-          [SMTPat (index sa i)] = 
+          [SMTPat (index sa i)] =
     lemma_unzip_index sab i;
     lemma_zip_index sa sb i
   in
   assert(equal sa (fst (unzip sab)));
   let aux2 (i:seq_index sb):
-    Lemma (requires (True)) 
+    Lemma (requires (True))
           (ensures (index sb i = index (snd (unzip sab)) i))
-          [SMTPat (index sb i)] = 
+          [SMTPat (index sb i)] =
     lemma_unzip_index sab i;
     lemma_zip_index sa sb i
-  in  
+  in
   assert(equal sb (snd (unzip sab)));
   ()
 
-let rec attach_index_aux (#a:Type) (s:seq a): Tot (seq (nat * a)) 
+let rec attach_index_aux (#a:Type) (s:seq a): Tot (seq (nat * a))
   (decreases (length s)) =
   let n = length s in
   if n = 0 then empty
@@ -645,13 +667,13 @@ let rec attach_index_aux (#a:Type) (s:seq a): Tot (seq (nat * a))
     let e = index s (n - 1) in
     let is' = attach_index_aux s' in
     append1 is' (n - 1, e)
-  
+
 let attach_index = attach_index_aux
 
 let rec lemma_attach_len_aux (#a:Type) (s: seq a):
   Lemma (requires (True))
         (ensures (length (attach_index s) = length s))
-        (decreases (length s)) = 
+        (decreases (length s)) =
   let n = length s in
   if n = 0 then ()
   else lemma_attach_len_aux (prefix s (n - 1))
@@ -660,10 +682,10 @@ let lemma_attach_len = lemma_attach_len_aux
 
 let rec lemma_attach_correct_aux (#a:Type) (s: seq a) (i: seq_index s):
   Lemma (requires (True))
-        (ensures (length (attach_index s) = length s /\        
+        (ensures (length (attach_index s) = length s /\
                   snd (index (attach_index s) i) == index s i /\
                   fst (index (attach_index s) i) = i))
-        (decreases (length s)) = 
+        (decreases (length s)) =
   lemma_attach_len s;
   let n = length s in
   if n = 0 then ()
@@ -672,27 +694,27 @@ let rec lemma_attach_correct_aux (#a:Type) (s: seq a) (i: seq_index s):
 
 let lemma_attach_correct = lemma_attach_correct_aux
 
-let rec reduce_aux (#a:Type) (#b:Type) (b0: b) (f: a -> b -> b) (s: seq a): 
-  Tot b (decreases (length s)) = 
+let rec reduce_aux (#a:Type) (#b:Type) (b0: b) (f: a -> b -> b) (s: seq a):
+  Tot b (decreases (length s)) =
   let n = length s in
   if n = 0 then b0
   else
     let s' = prefix s (n - 1) in
     let b' = reduce_aux b0 f s' in
     let e = index s (n - 1) in
-    f e b' 
+    f e b'
 
 let reduce = reduce_aux
 
 let lemma_reduce_empty (#a:Type) (#b:eqtype) (b0:b) (f:a -> b -> b):
   Lemma (reduce b0 f (empty #a) = b0) = ()
 
-let rec lemma_reduce_prefix_aux (#a:Type) (#b:eqtype) 
-                                (b0: b) (f: a -> b -> b) (s: seq a) 
+let rec lemma_reduce_prefix_aux (#a:Type) (#b:eqtype)
+                                (b0: b) (f: a -> b -> b) (s: seq a)
                                 (i:nat{i <= length s}):
   Lemma (requires True)
         (ensures (reduce b0 f s = reduce (reduce b0 f (prefix s i)) f (suffix s (length s - i))))
-        (decreases (length s)) = 
+        (decreases (length s)) =
   let n = length s in
   if n = 0 then ()
   else if i = n then ()
@@ -703,7 +725,7 @@ let lemma_reduce_prefix = lemma_reduce_prefix_aux
 let rec lemma_reduce_property_closure_aux (#a:Type) (#b:eqtype) (p: b -> bool) (b0:b) (f: a -> b -> b) (s: seq a):
   Lemma (requires (p b0 /\ (forall (x:a). forall (y:b). (p y ==> p (f x y)))))
         (ensures (p (reduce b0 f s)))
-        (decreases (length s)) = 
+        (decreases (length s)) =
   let n = length s in
   if n = 0 then ()
   else
@@ -713,7 +735,7 @@ let lemma_reduce_property_closure = lemma_reduce_property_closure_aux
 
 let lemma_reduce_identity (#a:Type) (#b:eqtype) (b0: b) (f: a -> b -> b) (s: seq a):
   Lemma (requires (forall (x:a). f x b0 = b0))
-        (ensures (reduce b0 f s = b0)) = 
+        (ensures (reduce b0 f s = b0)) =
   lemma_reduce_property_closure (fun y -> y = b0) b0 f s
 
 let lemma_reduce_singleton (#a:Type) (#b:eqtype) (b0: b) (f: a -> b -> b) (s: seq a{length s = 1}):
